Very minor work on Kennedy's translation

theories/Lambda/Kennedy.v
@@ -2,17 +2,19 @@
 (*   Copyright (c) 2019--2025 - Paulo Torrens <paulotorrens AT gnu DOT org>   *)
 (******************************************************************************)
 
+Require Import Lia.
 Require Import List.
 Require Import Equality.
 Require Import Local.Prelude.
 Require Import Local.AbstractRewriting.
 Require Import Local.Substitution.
+Require Import Local.Residuals.
 Require Import Local.Lambda.Calculus.
 Require Import Local.Lambda.PlotkinCBV.
 
 Import ListNotations.
 
-(* The naïve one-pass CPS translation of Danvy and Filinski's that Kennedy
+(* The naive one-pass CPS translation of Danvy and Filinski's that Kennedy
    describes in his paper is given as follows:
 
      [-]: term -> (var -> pseudoterm) -> pseudoterm
@@ -26,26 +28,26 @@ Import ListNotations.
                                   |     /|\
                                   +------+
 
-   This translation corresponds to Plotkin's CBV translation, of course. Also,
-   modulo a very minor change in application, the above is also used in Appel's
-   book (ch. 5), and it is given in Thielecke's thesis; namely, Appel's version
-   is given by changing the rule to:
+   This translation corresponds to Plotkin's CBV translation semantically, of
+   course. Also, modulo a very minor change in the application rule, the above
+   is also used in Appel's book (ch. 5.4), and it's given in Thielecke's thesis;
+   namely, Appel's version is given by changing application to:
 
-     [e1 e2] K = [e1] (\z1.
+     [e1 e2] K = [e1] (\z1.            (NOTE: k is outside the lambda now!)
                    [e2] (\z2.
                     z1<z2, k>)) { k<v> = K(v) }
 
-   ...which, clearly, doesn't change the meaning of the term. We use Kennedy's
-   version merely as the continuation is kept closer, so it's easier to deal
-   with (and it remains as de Bruijn index zero).
+   ...which, clearly, doesn't change the meaning of the term (assuming k fresh).
+   We use Kennedy's version merely as the continuation is immediately bound, so
+   it's easier to deal with (as it remains as de Bruijn index zero).
 
-   Kennedy provides an additional translation which we may also adapt, in that
-   tail-calls are optimized on the fly. This may be done by modifying the above
-   with the following rule:
+   Kennedy provides an additional translation later in this paper which we shall
+   also adapt, in that tail-calls are optimized on the fly. This may be done by
+   modifying the above with the following rule:
 
      [\x.e] K = K(f) { f<x, k> = (e) k }
 
-   Along with the introduction of an auxiliary, mutually defined definition:
+   Along with the introduction of an auxiliary, mutually defined function:
 
      (-): term -> var -> pseudoterm
 
@@ -53,55 +55,137 @@ Import ListNotations.
      (\x.e) k = k<f> { f<x, j> = (e) j }
      (e1 e2) k = [e1] (\z1.[e2] (\z2.z1<z2, k>))
 
-   We ignore that Kennedy's version is a so called double-barrelled translation,
-   in which he also gives an additional continuation for exception handlers.
+   We ignore that Kennedy's version is given as a so called double-barrelled
+   translation, in which he also gives an additional continuation for exception
+   handlers. Of course, we also ignored that Appel's version covers primitives.
 
    We would like to show that we can get from Plotkin's translation to the first
    one by performing administrative jumps, then from the that to the final one
-   by performing some tail-call eliminations. The combination would lead to the
+   by performing some shrinking reductions. The combination should lead to the
    result that these translations are adequate and that they give a sound
-   denotational semantics for the lambda calculus. Also, they may be helpful in
-   studying ANF, as this translation should eliminate administrative redexes. *)
+   denotational semantics for the lambda calculus. *)
 
-Local Definition tail: Type :=
-  nat -> nat -> CPS.pseudoterm -> Prop.
+Inductive kennedy_callback: Set :=
+  | kennedy_halt
+  | kennedy_call (f: nat) (t: CPS.pseudoterm) (c: CPS.pseudoterm).
 
-Local Definition halt: tail :=
-  fun k n b =>
-    b = CPS.jump (CPS.bound k) [CPS.bound (lift 1 k n)].
+Fixpoint kennedy_apply (K: kennedy_callback) (k n: nat): CPS.pseudoterm :=
+  match K with
+  (* (k, n) => k<n> *)
+  | kennedy_halt =>
+    CPS.jump (CPS.bound k) [CPS.bound (lift 1 k n)]
+  (* (k, n) => f<n, k> { k<v: t> = b } *)
+  | kennedy_call f t c =>
+    CPS.bind (CPS.jump (CPS.bound f) [CPS.bound k; CPS.bound (lift 1 k n)]) [t] c
+  end.
 
-Local Notation ABS b t1 t2 c :=
-  (CPS.bind b [t1; t2] c) (only parsing).
+Local Coercion kennedy_apply: kennedy_callback >-> Funclass.
 
-Inductive kennedy: term -> tail -> CPS.pseudoterm -> Prop :=
+Inductive kennedy: term -> kennedy_callback -> CPS.pseudoterm -> Prop :=
+  (* [x] K = K(x) *)
   | kennedy_bound:
-    (* [x] K = K(x)*)
-    forall K n b,
-    K 0 n b ->
-    kennedy (bound n) K b
+    forall K n,
+    (* Straightforward; the current continuation is 0 and thus everything else
+       gets shifted by 1 up. *)
+    kennedy (bound n) K (K 0 n)
+  (* [\x.e] K = K(f) { f<x, k> = [e] (\z.k<z>) } *)
   | kennedy_abstraction:
-    (* [\x.e] K = K(f) { f<x, k> = [e] (\z.k<z>) } *)
-    forall K t e b c,
-    K 1 0 b ->
-    kennedy e halt c ->
-    kennedy (abstraction t e) K (ABS b CPS.void CPS.void c)
+    forall K t e c,
+    (* We have to add the outer k variable to e; of course, we could also add
+       it after the translation if we'd deem fit. *)
+    kennedy (lift 1 1 e) kennedy_halt c ->
+    kennedy (abstraction t e) K (CPS.bind
+                                  (* The current continuation is 1, thus 0 here
+                                     is bound and refers to f. *)
+                                  (K 1 0)
+                                  [CPS.void; CPS.void]
+                                  (* Unchanged (we already added k). *)
+                                  c)
+  (* [f e] K = [f] (\f.
+                       [e] (\v.
+                               f<v, k> { k<x> = K(x) }
+                           )
+                   )
 
+      In the term f<v, k> { ... }, i.e., the anchor, both *)
   (* | kennedy_application:
-    (* [e1 e2] K = [e1] (\z1.[e2] (\z2. z1<z2, k> { k<v> = K(v) })) *) *).
+    forall (K: kennedy_callback) f e b c,
+    (* Oh boy, a tricky one... *)
+    kennedy (lift 2 0 e) (kennedy_call 0 CPS.void (K 0 1)) c ->
+    kennedy (lift 1 0 f) *)
+  .
 
 Goal
-  forall e b,
+  let e := (application 42 51) in
+  forall b c,
+  cbv_cps e b ->
+  kennedy e kennedy_halt c ->
+  Reduction.star b c.
+Proof.
+  compute; intros.
+  dependent destruction H.
+  vm_compute in H, H0.
+  dependent destruction H.
+  dependent destruction H0.
+  vm_compute.
+  eapply rt_trans.
+  apply rt_step.
+  apply Reduction.step_bind_right.
+  apply Reduction.step_ctxjmp with (h := Context.context_hole).
+  reflexivity.
+  vm_compute.
+  eapply rt_trans.
+  apply rt_step.
+  apply Reduction.step_bind_right.
+  apply Reduction.step_gc.
+  repeat constructor; auto.
+  vm_compute.
+  eapply rt_trans.
+  apply rt_step.
+  apply Reduction.step_ctxjmp with (h := Context.context_hole).
+  reflexivity.
+  vm_compute.
+  eapply rt_trans.
+  apply rt_step.
+  apply Reduction.step_gc.
+  repeat constructor; auto.
+  vm_compute.
+  admit.
+Admitted.
+
+Goal
+  forall t u n,
+  let e := (abstraction t (abstraction u (bound n))) in
+  forall b,
   cbv_cps e b ->
   forall c,
-  kennedy e halt c ->
-  Local.Reduction.conv b c.
+  kennedy e kennedy_halt c ->
+  b = c.
 Proof.
-  (* We'll obviously have to strengthen the inductive hypothesis... *)
-  induction 1; intros.
-  - dependent destruction H.
-    apply Local.Reduction.conv_refl.
-  - dependent destruction H0.
-    change (lift 1 1 0) with 0.
-    admit.
-  - admit.
-Admitted.
+  compute; intros.
+  dependent destruction H.
+  dependent destruction H.
+  destruct n.
+  vm_compute in H.
+  dependent destruction H.
+  dependent destruction H0.
+  dependent destruction H0.
+  dependent destruction H0.
+  vm_compute.
+  reflexivity.
+  destruct n.
+  vm_compute in H.
+  dependent destruction H.
+  dependent destruction H0.
+  dependent destruction H0.
+  dependent destruction H0.
+  vm_compute.
+  reflexivity.
+  vm_compute in H.
+  dependent destruction H.
+  dependent destruction H0.
+  dependent destruction H0.
+  dependent destruction H0.
+  vm_compute.
+  reflexivity.
+Qed.
